ground_zero/theorems/ua.lean
@@ -80,6 +80,9 @@ def is_zero : ℕ → bool
 example (h : 0 = 1) : empty :=
 ff_neq_tt (is_zero # h)⁻¹
 
+theorem succ_neq_zero (n : ℕ) (h : nat.succ n = 0) : empty :=
+ff_neq_tt (is_zero # h)
+
 def neg_bool_equiv : bool ≃ bool := begin
   existsi bnot, split; existsi bnot; intro x; simp
 end
