ground_zero/types/coproduct.lean
@@ -4,15 +4,15 @@ namespace ground_zero.types
 
 universes u v f
 
-inductive coproduct (α : Type u) (β : Type v)
+inductive coproduct (α : Sort u) (β : Sort v)
 | inl {} : α → coproduct
 | inr {} : β → coproduct
 infix ` + ` := coproduct
 
 namespace coproduct
-  variables {α : Type u} {β : Type v}
+  variables {α : Sort u} {β : Sort v}
 
-  def elim {γ : Type f} (g₀ : α → γ) (g₁ : β → γ) : α + β → γ
+  def elim {γ : Sort f} (g₀ : α → γ) (g₁ : β → γ) : α + β → γ
   | (inl a) := g₀ a
   | (inr b) := g₁ b
 
